Differentiate concat of list, strings, and bytearrays

lean4/Verification/Basic.lean
@@ -138,26 +138,26 @@ def merge {α : Type} (r : α → α → Bool)
   | l, [] => l
   | a :: l, b :: l' => if (r a b) then a :: merge r l (b :: l') else b :: merge r (a :: l) l'
 
-def mergeSort (r : α → α → Bool) : List α → List α
+def merge_sort (r : α → α → Bool) : List α → List α
   | [] => []
   | [a] => [a]
   | a :: b :: l => by
-    -- Porting note: rewrote to make `mergeSort_cons_cons` proof easier
+    -- Porting note: rewrote to make `merge_sort_cons_cons` proof easier
     let ls := (split (a :: b :: l))
     have e : split (a :: b :: l) = ⟨ls.1, ls.2⟩ := rfl
     have h := length_split_lt e
     have := h.1
     have := h.2
-    exact merge r (mergeSort r ls.1) (mergeSort r ls.2)
+    exact merge r (merge_sort r ls.1) (merge_sort r ls.2)
   termination_by l => length l
 
--- This is mergeSort_cons_cons from the mathlib library
+-- This is merge_sort_cons_cons from the mathlib library
 
 theorem sort_correctness {a b} {c xs ys : List α} (r : α → α → Bool)
     (h : split (a :: b :: c) = (xs, ys)) :
-    mergeSort r (a :: b :: c) = merge r (mergeSort r xs) (mergeSort r ys) := 
+    merge_sort r (a :: b :: c) = merge r (merge_sort r xs) (merge_sort r ys) := 
   by
-  simp only [mergeSort, h]
+  simp only [merge_sort, h]
 
 
 /- In sort, length is the same as the length of the sorted input -/
@@ -206,32 +206,45 @@ theorem sort_equal_length {α : Type} (sort : (α → α → Bool) → List α �
   The grep_agg function is a simple aggregation function that concatenates the results of two greps.
 -/
 
-def concat : String → String → String :=
+def concat_string : String → String → String :=
   λ x y ↦ x ++ y
 
-theorem concat_correctness 
+theorem concat_string_correctness 
   (f : String → String) 
   (xs ys : String) 
   (h : ∀ xs ys, f (xs ++ ys) = f xs ++ f ys) : 
-  f (xs ++ ys) = concat (f xs) (f ys) :=
+  f (xs ++ ys) = concat_string (f xs) (f ys) :=
   by
-    rw [concat]
+    rw [concat_string]
     rw [h]
 
 -- Cat is just a function that concatenates two strings
-theorem cat_size
+theorem catSize
   (cat : String → String)
   (h : ∀ s xs ys, s = xs ++ ys → cat s = cat xs ++ cat ys) : 
   ∀ s xs ys a b c d, 
     s = xs ++ ys → 
     xs = a ++ b →
     ys = c ++ d →
-    concat (cat xs) (cat ys) = concat (cat a) (cat b) ++ concat (cat c) (cat d) := 
+    concat_string (cat xs) (cat ys) = concat_string (cat a) (cat b) ++ concat_string (cat c) (cat d) := 
   by
     intro s xs ys a b c d a_1 a_2 a_3
     subst a_3 a_1 a_2
     simp_all only
     rfl
+
+-- The actual Concat function is a ByteArray
+def concat_bytearray (acc x : ByteArray) : ByteArray := 
+  acc ++ x
+
+theorem concat_bytearray_correctness
+  (f : ByteArray → ByteArray) 
+  (xs ys : ByteArray) 
+  (h : ∀ xs ys, f (xs ++ ys) = f xs ++ f ys) : 
+  f (xs ++ ys) = concat_bytearray (f xs) (f ys) :=
+  by
+    rw [concat_bytearray]
+    rw [h]
 
 def concat_list : List String → List String → List String :=
   λ xs ys ↦ xs ++ ys
@@ -264,7 +277,7 @@ theorem grep_size
     exact Nat.add_le_add h₁ h₂
 
 -- Membership is preserved
-theorem grep_contains
+theorem grep_membership
   (grep: List String → String → List String)
   (h: ∀ lines pattern, ∀ line ∈ (grep lines pattern), line ∈ lines) :
   ∀ lines pattern, 
@@ -314,26 +327,26 @@ def uniq_uniq {α : Type} [DecidableEq α] (xs ys: List α) :
         -- rw [ih]
         -- simp
 
-def uniq_aggregator (xs ys : List String)  : List String :=
+def uniq_merge (xs ys : List String)  : List String :=
   match xs, ys with 
   | [], ys => ys
   | xs, [] => xs
   | x :: xs, y :: ys =>
-    if x == y then x :: uniq_aggregator xs ys
-    else x :: uniq_aggregator xs (y :: ys)
+    if x == y then x :: uniq_merge xs ys
+    else x :: uniq_merge xs (y :: ys)
 
-theorem uniq_agg_size : ∀ a b, (uniq_aggregator a b).length <= a.length + b.length := 
+theorem uniq_merge_size : ∀ a b, (uniq_merge a b).length <= a.length + b.length := 
   by
     intro a b
     induction a generalizing b with
       | nil => 
-        simp [uniq_aggregator]
+        simp [uniq_merge]
       | cons x xs ih =>
         induction b with
           | nil =>
-            simp [uniq_aggregator]
+            simp [uniq_merge]
           | cons y ys ih2 =>
-            simp [uniq_aggregator]
+            simp [uniq_merge]
             split_ifs
             case pos =>
               simp [List.length_cons]
@@ -350,16 +363,16 @@ theorem uniq_size (uniq: List String → List String)
   (h: ∀ lines, (uniq lines).length <= lines.length) :
   ∀ lines, 
     ∀ a b, lines = a ++ b → 
-    (uniq_aggregator (uniq a) (uniq b)).length <= lines.length := 
+    (uniq_merge (uniq a) (uniq b)).length <= lines.length := 
   by
     intro lines a b hsplit 
     have h₁ := h a
     have h₂ := h b
-    have h₃ := uniq_agg_size (uniq a) (uniq b)
+    have h₃ := uniq_merge_size (uniq a) (uniq b)
     rw [hsplit]
     simp [List.length_append]
     calc
-      (uniq_aggregator (uniq a) (uniq b)).length
+      (uniq_merge (uniq a) (uniq b)).length
           ≤ (uniq a).length + (uniq b).length := h₃
       _ ≤ a.length + b.length := by
         apply add_le_add
@@ -370,20 +383,20 @@ theorem uniq_size (uniq: List String → List String)
     subst hsplit
     simp_all only [List.length_append, le_refl]
 
-theorem uniq_aggregator_contains : ∀ a b, ∀ line ∈ uniq_aggregator a b, line ∈ a ++ b := 
+theorem uniq_merge_membership : ∀ a b, ∀ line ∈ uniq_merge a b, line ∈ a ++ b := 
   by
     intro a b line hin
     induction a generalizing b with
       | nil => 
-        simp [uniq_aggregator] at hin
+        simp [uniq_merge] at hin
         exact hin
       | cons x xs ih =>
         induction b with
           | nil =>
-            simp [uniq_aggregator] at hin
+            simp [uniq_merge] at hin
             simp [hin]
           | cons y ys ih2 =>
-            simp [uniq_aggregator] at hin
+            simp [uniq_merge] at hin
             simp [List.cons_append]
             split_ifs at hin with h_eq
             case pos =>
@@ -415,16 +428,16 @@ theorem uniq_aggregator_contains : ∀ a b, ∀ line ∈ uniq_aggregator a b, li
                   simp_all only [List.mem_append, List.cons_append, List.mem_cons]
 
 -- Membership is preserved
-theorem uniq_contains
+theorem uniq_membership
   (uniq: List String → List String)
   (h: ∀ lines, ∀ line ∈ (uniq lines), line ∈ lines) :
   ∀ lines, 
     ∀ a b, lines = a ++ b → 
-      ∀ line ∈ (uniq_aggregator (uniq a) (uniq b)), line ∈ lines := 
+      ∀ line ∈ (uniq_merge (uniq a) (uniq b)), line ∈ lines := 
   by
     intro lines a b hsplit line hin
     rw [hsplit]
-    have hcontains := uniq_aggregator_contains (uniq a) (uniq b) line hin
+    have hcontains := uniq_merge_membership (uniq a) (uniq b) line hin
     cases List.mem_append.1 hcontains with
     | inl huniqa =>
       have ha := h a line huniqa
